Add Gthunks.v, implementing a derived API for thunks-with-generation-ids
.. and update the proof of pqueue to use it

theories/pqueue/Proof.v
@@ -3,7 +3,7 @@ From iris.base_logic.lib Require Import na_invariants.
 From iris.algebra Require Import auth excl agree csum.
 From iris_time.heap_lang Require Import proofmode notation.
 From iris_time.heap_lang Require Import notation.
-From iris_time Require Import TimeCredits Thunks Auth_max_nat.
+From iris_time Require Import TimeCredits Gthunks Auth_max_nat.
 From iris_time.pqueue Require Import Code.
 
 Fixpoint list_val (l : list val) : val :=
@@ -11,26 +11,6 @@ Fixpoint list_val (l : list val) : val :=
   | nil => #()
   | x :: l' => (x, list_val l')
   end.
-
-Definition ns (n : nat) : namespace :=
-  nroot .@ "pqueue" .@ n.
-
-Fixpoint nset (n : nat) : coPset :=
-  match n with
-  | 0 => ∅
-  | S n' => nset n' ∪ ↑(ns n')
-  end.
-
-Lemma ns_nset_disj n n' :
-  n ≤ n' →
-  ↑ns n' ## nset n.
-Proof.
-  revert n'; induction n; cbn; intros n'.
-  - set_solver.
-  - intros Hn'. rewrite disjoint_union_r. split.
-    + eapply IHn. lia.
-    + unfold ns. assert (n ≠ n') by lia. solve_ndisj.
-Qed.
 
 Section PQueue.
 
@@ -103,15 +83,13 @@ Definition is_queue_raw
   (q : val)
   (l w fl rl : list val) : iProp Σ
 :=
-  ∃ (t : loc) (lenf lenr : nat) (γ : gname) (ns_id : nat),
+  ∃ (t : loc) (lenf lenr : nat) (γ : gname) (id : genid),
     ⌜q = (list_val w, #lenf, #t, #lenr, list_val rl)%V
      ∧ lenf = length fl
      ∧ lenr = length rl
      ∧ l = fl ++ reverse rl
      ∧ w `prefix_of` fl⌝ ∗
-    Thunk p (ns ns_id) γ t
-          (thunk_debt w fl rl)
-          (na_own p (nset ns_id))
+    Gthunk p id γ t (thunk_debt w fl rl)
           (λ fv, ⌜fv = list_val fl⌝).
 
 Definition is_queue (q : val) (l : list val) : iProp Σ :=
@@ -134,8 +112,7 @@ Proof using.
   wp_tick_lam. wp_tick_closure.
   rewrite (_: 8 = 4 + 4) //. iDestruct "TC" as "[TC1 TC]".
   iDestruct "TC1" as "[TC11 TC12]".
-  iPoseProof (create_spec _ (ns 0) (thunk_debt nil nil nil)
-                          (na_own p (nset 0))
+  iPoseProof (create_spec _ 0 (thunk_debt nil nil nil)
                           (λ flv', ⌜flv' = list_val nil⌝)%I
                           (λ: <>, list_val nil)%V
              with "[//] [$TC12 TC11]") as "S".
@@ -152,37 +129,31 @@ Qed.
    if [f] is empty. *)
 Lemma checkw_spec q l w fl rl :
   TC_invariant -∗
-  {{{ is_queue_raw q l w fl rl ∗ TC 44 ∗ na_own p ⊤ }}}
+  {{{ is_queue_raw q l w fl rl ∗ TC 44 ∗ own_gens_upto p None }}}
     «checkw q»
   {{{ q' w', RET «q'»;
-      is_queue_raw q' l w' fl rl ∗ na_own p ⊤
+      is_queue_raw q' l w' fl rl ∗ own_gens_upto p None
       ∗ ⌜w' = [] → fl = []⌝ }}}.
 Proof using.
-  iIntros "#Htickinv !#" (Φ) "(#Hq & TC & Hna) HΦ".
+  iIntros "#Htickinv !#" (Φ) "(#Hq & TC & Hgens) HΦ".
   iDestruct "Hq" as (t ? ? ? ns_id) "[(-> & -> & -> & -> & %) HT]".
   wp_tick_lam.
   repeat (wp_tick_let; repeat wp_tick_proj).
   destruct w as [|? w'] eqn:Hw.
   { wp_tick_op. wp_tick_if.
     rewrite (_: 15 = 11 + 4) //. iDestruct "TC" as "[TC1 TC]".
-    assert ((⊤:coPset) = nset ns_id ∪ (⊤ ∖ nset ns_id)) as Hsplit_top.
-    { apply union_difference_L. set_solver. }
-    rewrite {1}Hsplit_top. iDestruct (na_own_union with "Hna") as "[HnaT Hna]".
-    { set_solver. }
-    wp_apply (force_spec with "[//] [$HT $Hna $TC1 $HnaT]").
-    { apply subseteq_difference_r. 2: set_solver. by apply ns_nset_disj. }
-    iIntros (fv) "(TV & -> & Hna & HnaT)". repeat wp_tick_pair.
+    wp_apply (force_spec with "[//] [$HT $Hgens $TC1]"). done.
+    iIntros (fv) "(TV & -> & Hgens)". repeat wp_tick_pair.
     iApply ("HΦ" $! (list_val fl, #(length fl), #t, #(length rl), list_val rl)%V fl).
-    iDestruct (na_own_union with "[$HnaT $Hna]") as "Hna". set_solver.
-    rewrite -Hsplit_top. iFrame "Hna". iSplit.
-    { iExists _, _, _, _, _. iSplit; [done|]. iApply (Thunk_weaken with "HT").
+    iFrame "Hgens". iSplit.
+    { iExists _, _, _, _, _. iSplit; [done|]. iApply (Gthunk_weaken with "HT").
       unfold thunk_debt; lia. }
     done. }
   { wp_tick_op. wp_tick_if. repeat wp_tick_pair.
     iApply ("HΦ" $! (list_val (v::w'), #(length fl), #t, #(length rl), list_val rl)%V w).
-    iFrame "Hna". iSplit.
+    iFrame "Hgens". iSplit.
     { iExists _, _, _, _, _. rewrite -Hw. iSplit; [subst w; done|].
-      iApply (Thunk_weaken with "HT"). lia. }
+      iApply (Gthunk_weaken with "HT"). lia. }
     { iPureIntro. intros ->; inversion Hw. } }
 Qed.
 
@@ -192,15 +163,15 @@ Qed.
 Lemma check_spec q l w fl rl :
   length rl ≤ length fl + 1 →
   TC_invariant -∗
-  {{{ is_queue_raw q l w fl rl ∗ TC 121 ∗ na_own p ⊤ }}}
+  {{{ is_queue_raw q l w fl rl ∗ TC 121 ∗ own_gens_upto p None }}}
     «check q»
   {{{ q' w' fl' rl', RET «q'»;
       is_queue_raw q' l w' fl' rl'
       ∗ ⌜length rl' ≤ length fl'⌝
       ∗ ⌜w' = [] → fl' = []⌝
-      ∗ na_own p ⊤ }}}.
+      ∗ own_gens_upto p None }}}.
 Proof using.
-  intros Hlen. iIntros "#Htickinv !#" (Φ) "(#Hq & TC & Hna) HΦ".
+  intros Hlen. iIntros "#Htickinv !#" (Φ) "(#Hq & TC & Hgens) HΦ".
   iDestruct "Hq" as (t ? ? ? ns_id) "[(-> & -> & -> & -> & %) HT]".
   wp_tick_lam.
   repeat (wp_tick_let; repeat wp_tick_proj).
@@ -209,31 +180,25 @@ Proof using.
   { rewrite bool_decide_eq_true_2; [| lia]. wp_tick_if.
     rewrite (_: 92 = 44 + 48) //. iDestruct "TC" as "[TC1 TC]".
     wp_apply (checkw_spec (list_val w, #(length fl), #t, #(length rl), list_val rl)%V
-               with "[//] [$TC1 $Hna]").
+               with "[//] [$TC1 $Hgens]").
     { iExists _, _, _, _, _. iSplit. done. iFrame "HT". }
     iIntros (q' w') "(Hq' & Hna & %)". iApply "HΦ". by iFrame. }
   { rewrite bool_decide_eq_false_2; [| lia]. wp_tick_if.
     rewrite (_: 92 = 11 + 81) //. iDestruct "TC" as "[TC1 TC]".
     rewrite (_: thunk_debt w fl rl = 0).
     2: { rewrite /thunk_debt (_: 8 * length fl - 8 * length rl = 0)%nat; lia. }
-    assert ((⊤:coPset) = nset ns_id ∪ (⊤ ∖ nset ns_id)) as Hsplit_top.
-    { apply union_difference_L. set_solver. }
-    rewrite {1}Hsplit_top. iDestruct (na_own_union with "Hna") as "[HnaT Hna]".
-    { set_solver. }
-    wp_apply (force_spec with "[//] [$HT $Hna $TC1 $HnaT]").
-    { apply subseteq_difference_r. 2: set_solver. by apply ns_nset_disj. }
-    iIntros (flv) "(? & -> & Hna & HnaT)". wp_tick_let.
+    wp_apply (force_spec with "[//] [$HT $Hgens $TC1]"). done.
+    iIntros (flv) "(? & -> & Hgens)". wp_tick_let.
     wp_tick_closure.
     rewrite (_: 78 = 3 + 75) //. iDestruct "TC" as "[TC1 TC]".
     rewrite (_: 75 = S (5 + (6 + 8)) + 55) //. iDestruct "TC" as "[TC2 TC]".
     (* we can assign namespace id 0 to this thunk as it doesn't need to force
        other thunks. *)
-    iPoseProof (create_spec _ (ns 0) (16 * length fl)
-                            (na_own p (nset 0))
+    iPoseProof (create_spec _ 0 (16 * length fl)
                             (λ flv', ⌜flv' = list_val (fl ++ reverse rl)⌝)%I
                             (λ: <>, append (list_val fl) (rev (list_val rl)))%V
                with "[//] [$TC1 TC2]") as "S".
-    { iIntros "TC HnaT" (ψ) "Hψ". wp_tick_lam.
+    { iIntros "TC Hgens" (ψ) "Hψ". wp_tick_lam.
       rewrite (_: 16 * length fl = 8 * length fl + 8 * length fl); [|lia].
       iDestruct "TC" as "[TCa TCr]". iDestruct "TC2" as "[TC2 TCrc]".
       iCombine "TCrc TCr" as "TCr".
@@ -241,61 +206,60 @@ Proof using.
       iIntros (rrl) "->".
       iCombine "TC2 TCa" as "TCa".
       wp_apply (append_spec with "[//] [$TCa]").
-      iIntros (l') "->". by iApply ("Hψ" with "HnaT"). }
+      iIntros (l') "->". by iApply ("Hψ" with "Hgens"). }
     rewrite -lock. (* XXX *) wp_apply "S".
     iIntros (? t') "#HT'". wp_tick_let. wp_tick_op. repeat wp_tick_pair.
     rewrite (_: 48 = 44 + 4) //. iDestruct "TC" as "[TC1 TC]".
-    iDestruct (na_own_union with "[$HnaT $Hna]") as "Hna". set_solver. rewrite -Hsplit_top.
     wp_apply (checkw_spec (list_val fl, #(length fl + length rl), #t', #0, #())%V
                           (fl ++ reverse rl) fl (fl ++ reverse rl) nil
-               with "[//] [$TC1 $Hna]").
+               with "[//] [$TC1 $Hgens]").
     { iExists _, (length fl + length rl), 0, _, 0. iSplit. iPureIntro. split.
       - repeat f_equal. lia.
       - rewrite app_length reverse_length app_nil_r. repeat split. by apply prefix_app_r.
-      - iApply (Thunk_weaken with "HT'"). rewrite /thunk_debt.
+      - iApply (Gthunk_weaken with "HT'"). rewrite /thunk_debt.
         rewrite app_length reverse_length Nat.sub_0_r. lia. }
-    iIntros (q' w') "(Hq' & Hna & %)". iApply "HΦ". iFrame. iPureIntro; split; try done.
+    iIntros (q' w') "(Hq' & Hgens & %)". iApply "HΦ". iFrame. iPureIntro; split; try done.
     rewrite app_length reverse_length /=. lia. }
 Qed.
 
 Lemma push_spec q l x :
   TC_invariant -∗
-  {{{ is_queue q l ∗ TC 170 ∗ na_own p ⊤ }}}
+  {{{ is_queue q l ∗ TC 170 ∗ own_gens_upto p None }}}
     «push q x»
-  {{{ q', RET «q'»; is_queue q' (l ++ [x]) ∗ na_own p ⊤ }}}.
+  {{{ q', RET «q'»; is_queue q' (l ++ [x]) ∗ own_gens_upto p None }}}.
 Proof using.
-  iIntros "#Htickinv !#" (Φ) "(#Hq & TC & Hna) HΦ".
+  iIntros "#Htickinv !#" (Φ) "(#Hq & TC & Hgens) HΦ".
   iDestruct "Hq" as (w fl rl) "(Hqr & % & %)".
   iDestruct "Hqr" as (t ? ? ? ns_id) "[(-> & -> & -> & -> & %) HT]".
   wp_tick_lam. repeat (wp_tick_let; repeat wp_tick_proj).
   wp_tick_pair. wp_tick_op. repeat wp_tick_pair.
   rewrite (_: 135 = 8 + 127) //. iDestruct "TC" as "[TC1 TC]".
-  iDestruct (Thunk_pay with "TC1 HT") as ">#HT'". done.
+  iDestruct (Gthunk_pay with "TC1 HT") as ">#HT'". done.
   rewrite (_: 127 = 121 + 6) //. iDestruct "TC" as "[TC1 TC]".
   wp_apply (check_spec (list_val w, #(length fl), #t, #(length rl + 1), list_val (x::rl))%V
                        (fl ++ reverse rl ++ [x]) w fl (x :: rl)
-            with "[//] [$TC1 $Hna]").
+            with "[//] [$TC1 $Hgens]").
   { cbn; lia. }
   { iExists _, (length fl), (length rl + 1), _, _. iSplit. iPureIntro. split.
     - repeat f_equal. lia.
     - repeat split; auto. cbn; lia. rewrite reverse_cons //.
-    - iApply (Thunk_weaken with "HT'"). cbn; lia. }
-  iIntros (q' w' fl' rl') "(Hq' & % & % & Hna)". iApply "HΦ".
-  iFrame "Hna". rewrite app_assoc //. iExists _, _, _. by iFrame "Hq'".
+    - iApply (Gthunk_weaken with "HT'"). cbn; lia. }
+  iIntros (q' w' fl' rl') "(Hq' & % & % & Hgens)". iApply "HΦ".
+  iFrame "Hgens". rewrite app_assoc //. iExists _, _, _. by iFrame "Hq'".
 Qed.
 
 Lemma pop_spec q l :
   TC_invariant -∗
-  {{{ is_queue q l ∗ TC 250 ∗ na_own p ⊤ }}}
+  {{{ is_queue q l ∗ TC 250 ∗ own_gens_upto p None }}}
     «pop q»
   {{{ r, RET «r»;
       match l with
       | nil => ⌜r = NONEV⌝
       | x :: l' => ∃ q', ⌜r = SOMEV (x, q')%V⌝ ∗ is_queue q' l'
       end ∗
-      na_own p ⊤ }}}.
+      own_gens_upto p None }}}.
 Proof using.
-  iIntros "#Htickinv !#" (Φ) "(#Hq & TC & Hna) HΦ".
+  iIntros "#Htickinv !#" (Φ) "(#Hq & TC & Hgens) HΦ".
   iDestruct "Hq" as (w fl rl) "(Hqr & %Hlen & %Hw)".
   iDestruct "Hqr" as (t ? ? ? ns_id) "[(-> & -> & -> & -> & %Hpref) HT]".
   wp_tick_lam. repeat (wp_tick_let; repeat wp_tick_proj).
@@ -303,7 +267,7 @@ Proof using.
   { wp_tick_op. wp_tick_if. wp_tick_inj.
     rewrite Hw // (nil_length_inv rl) //.
     2: { rewrite Hw // in Hlen. cbn in Hlen. lia. }
-    cbn. iApply ("HΦ" $! (InjLV #())%V). by iFrame "Hna". }
+    cbn. iApply ("HΦ" $! (InjLV #())%V). by iFrame "Hgens". }
   { destruct fl as [|y fl]. by apply prefix_nil_not in Hpref.
     pose proof (prefix_cons_inv_1 _ _ _ _ Hpref). subst y.
     apply prefix_cons_inv_2 in Hpref.
@@ -313,41 +277,36 @@ Proof using.
     rewrite (_: 211 = 29 + 182) //. iDestruct "TC" as "[TC2 TC]".
     (* pick a new namespace id: we need to be able to force the thunk we are
        wrapping, and all the thunks it may then need to force. *)
-    iPoseProof (create_spec _ (ns (S ns_id)) (thunk_debt w' fl rl)
-                            (na_own p (nset (S ns_id)))
+    iPoseProof (create_spec _ (S ns_id) (thunk_debt w' fl rl)
                             (λ flv, ⌜flv = list_val fl⌝)%I
-                            (λ: <>, Snd (force #t))%V
+                            (λ: <>, Snd (Thunks.force #t))%V
                with "[//] [$TC1 TC2]") as "S".
-    { iIntros "TC HnaT" (ψ) "Hψ". wp_tick_lam.
+    { iIntros "TC Hgens" (ψ) "Hψ". wp_tick_lam.
       rewrite (_: 28 = 12 + 16) //. iDestruct "TC2" as "[TC1 TC2]".
       iCombine "TC2 TC" as "TC".
-      iDestruct (Thunk_pay _ _ _ _ _ _ (thunk_debt (x :: w') (x :: fl) rl)
-                           with "[TC] HT") as ">#HTpaid". done.
+      iDestruct (Gthunk_pay _ _ _ _ _ _ (thunk_debt (x :: w') (x :: fl) rl)
+                            with "[TC] HT") as ">#HTpaid". done.
       { iApply (TC_weaken with "TC"). rewrite /thunk_debt.
         rewrite !(_: ∀ x l, length (x :: l) = S (length l)); [|done..]. lia. }
       rewrite Nat.sub_diag.
 
-      cbn [nset]. iDestruct (na_own_union with "HnaT") as "[HnaT Hna]".
-      { symmetry; by apply ns_nset_disj. }
-
       iDestruct "TC1" as "[TC1 TC2]".
-      wp_apply (force_spec with "[//] [$TC2 $HTpaid $Hna $HnaT]"). done.
-      iIntros (flv) "(_ & -> & Hna & HnaT)". rewrite /=. wp_tick_proj.
-      iApply ("Hψ" with "[Hna HnaT]"). iApply (na_own_union with "[$HnaT $Hna]").
-      symmetry; by apply ns_nset_disj. done. }
+      wp_apply (force_spec with "[//] [$TC2 $HTpaid $Hgens]"). cbn; lia.
+      iIntros (flv) "(_ & -> & Hgens)". rewrite /=. wp_tick_proj.
+      by iApply ("Hψ" with "Hgens"). }
     rewrite -lock. (* XXX *) wp_apply "S". iIntros (? t') "#HT'".
     wp_tick_let. wp_tick_op. repeat wp_tick_pair.
     rewrite (_: 175 = 121 + 54) //. iDestruct "TC" as "[TC1 TC]".
     wp_apply (check_spec (list_val w', #(S (length fl) - 1), #t', #(length rl), list_val rl)%V
                          (fl ++ reverse rl) w' fl rl
-               with "[//] [$TC1 $Hna]").
+               with "[//] [$TC1 $Hgens]").
     { cbn in Hlen; lia. }
     { iExists _, _, _, _, _. iSplit. iPureIntro. repeat split; auto.
       - repeat f_equal. lia.
       - iFrame "HT'". }
-    iIntros (q' w'' fl' rl') "(Hq' & % & % & Hna)".
+    iIntros (q' w'' fl' rl') "(Hq' & % & % & Hgens)".
     wp_tick_let. wp_tick_pair. wp_tick_inj.
-    cbn [app]. iApply ("HΦ" $! (InjRV (x, q')%V)). iFrame "Hna".
+    cbn [app]. iApply ("HΦ" $! (InjRV (x, q')%V) with "[$Hgens Hq']").
     iExists q'. iSplit; first done. iExists _, _, _. by iFrame. }
 Qed.
 
