theories/Gthunks.v
@@ -1,0 +1,152 @@
+From stdpp Require Import namespaces.
+From iris.base_logic.lib Require Import na_invariants.
+From iris.algebra Require Import auth excl agree csum.
+From iris_time Require Import TimeCredits Auth_max_nat Thunks.
+
+Definition genid := nat.
+
+Definition gen_ns (id : genid) : namespace :=
+  nroot .@ "gthunk" .@ id.
+
+(* auxiliary definition *)
+Fixpoint gens_upto' (id : genid) : coPset :=
+  match id with
+  | O => ∅
+  | S id' => gens_upto' id' ∪ ↑(gen_ns id')
+  end.
+
+(* A set of generations.
+   If the bound is [Some id], this corresponds to the set [0, id);
+   If the bound is [None], then this corresponds to [0, +oo). *)
+Definition gens_upto (bound : option genid) : coPset :=
+  match bound with
+  | None => ⊤
+  | Some id => gens_upto' id
+  end.
+
+(* Compare an identifier with a bound. In other words, this checks whether the
+   generation [id] is in the set [gens_upto bound]. *)
+Definition is_upto (id : genid) (bound : option genid) : Prop :=
+  match bound with
+  | None => True
+  | Some id' => id < id'
+  end.
+
+Lemma gen_ns_disj_upto' (n n' : genid) :
+  n ≤ n' →
+  ↑gen_ns n' ## gens_upto' n.
+Proof.
+  revert n'; induction n; cbn; intros n'.
+  - set_solver.
+  - intros Hn'. rewrite disjoint_union_r. split.
+    + eapply IHn. lia.
+    + unfold gen_ns. assert (n ≠ n') by lia. solve_ndisj.
+Qed.
+
+Lemma gens_upto'_mono (id id' : genid) :
+  id ≤ id' →
+  gens_upto' id ⊆ gens_upto' id'.
+Proof.
+  revert id; induction id'; intros id Hid; cbn.
+  - assert (id = 0) by lia; by subst id.
+  - destruct (decide (id = S id')).
+    + subst id. cbn. done.
+    + specialize (IHid' id ltac:(lia)). set_solver.
+Qed.
+
+Lemma gen_ns_sub_upto (id id' : genid) :
+  id < id' →
+  ↑gen_ns id ⊆ gens_upto' id'.
+Proof.
+  intros Hid.
+  assert (HH: ↑gen_ns id ⊆ gens_upto' (S id)).
+  { cbn. set_solver. }
+  transitivity (gens_upto' (S id)); auto.
+  by apply gens_upto'_mono.
+Qed.
+
+Section Gthunks.
+
+  Notation valO := (valO heap_lang).
+  Context `{timeCreditHeapG Σ}.
+  Context `{inG Σ (csumR (exclR unitO) (agreeR valO))}. (* γ *)
+  Context `{inG Σ (authR $ optionUR $ exclR boolO)}.    (* γforced *)
+  Context `{inG Σ (authR max_natUR)}.                   (* γpaid *)
+  Context `{na_invG Σ}.
+
+  Implicit Type p : na_inv_pool_name.
+  Implicit Type id : genid.
+  Implicit Type γ : gname.
+  Implicit Type t : loc.
+  Implicit Type n m k : nat.
+  Implicit Type f : val.
+
+  Definition own_gens_upto p (bound : option genid) :=
+    na_own p (gens_upto bound).
+
+  Lemma own_gens_upto_alloc : ⊢ |==> ∃ p, own_gens_upto p None.
+  Proof using. iApply na_alloc. Qed.
+
+  Definition Gthunk p id γ t n φ : iProp Σ :=
+    Thunk p (gen_ns id) γ t n
+            (own_gens_upto p (Some id)) φ.
+
+  Instance Gthunk_persistent p id γ t n φ :
+    Persistent (Gthunk p id γ t n φ).
+  Proof using. exact _. Qed.
+
+  Lemma Gthunk_weaken p id γ t n₁ n₂ φ :
+    (n₁ ≤ n₂)%nat →
+    Gthunk p id γ t n₁ φ -∗
+    Gthunk p id γ t n₂ φ.
+  Proof using. iIntros (?) "H". by iApply Thunk_weaken. Qed.
+
+  Lemma Gthunk_consequence p id γ t n m φ ψ :
+    (∀ v, TC m -∗ φ v ={⊤}=∗ □ ψ v) -∗
+    Gthunk p id γ t  n    φ  ={∅}=∗
+    Gthunk p id γ t (n+m) ψ.
+  Proof using. iIntros "H1 H2". by iMod (Thunk_consequence with "H1 H2"). Qed.
+
+  Lemma Gthunk_pay E p id γ t n k φ :
+    ↑thunkPayN t ⊆ E →
+    TC k -∗ Gthunk p id γ t n φ ={E}=∗ Gthunk p id γ t (n-k) φ.
+  Proof using. iIntros (?) "H1 H2". by iMod (Thunk_pay with "H1 H2"). Qed.
+
+  Lemma create_spec p id n φ f :
+    TC_invariant -∗
+    {{{ TC 3 ∗ ( TC n -∗ own_gens_upto p (Some id) -∗
+                 ∀ ψ, (∀ v, own_gens_upto p (Some id) -∗ □ φ v -∗ ψ «v»%V) -∗
+                 WP «f #()» {{ ψ }} ) }}}
+    « create f »
+    {{{ γ t, RET #t ; Gthunk p id γ t n φ }}}.
+  Proof using.
+    iIntros "#HtickInv" (Φ) "!# H Post".
+    by wp_apply (Thunks.create_spec with "HtickInv H").
+  Qed.
+
+  Lemma force_spec p id bound γ t φ :
+    is_upto id bound →
+    TC_invariant -∗
+    {{{ TC 11 ∗ Gthunk p id γ t 0 φ ∗ own_gens_upto p bound }}}
+    « force #t »
+    {{{ v, RET «v» ; ThunkVal γ v ∗ □ φ v ∗ own_gens_upto p bound }}}.
+  Proof using.
+    intros Hid. iIntros "#HtickInv" (Φ) "!# (TC & H & Hgens) HΦ".
+    rewrite /own_gens_upto.
+    assert (gens_upto bound = gens_upto' id ∪ (gens_upto bound ∖ gens_upto' id)) as Hsplit_gens.
+    { apply union_difference_L. destruct bound.
+      + apply gens_upto'_mono. cbn in Hid. lia.
+      + cbn. set_solver. }
+    rewrite Hsplit_gens. iDestruct (na_own_union with "Hgens") as "[Hgens Hthunk]".
+    { set_solver. }
+    assert (↑gen_ns id ⊆ gens_upto bound ∖ gens_upto' id) as Hthunk.
+    { apply subseteq_difference_r. by apply gen_ns_disj_upto'. destruct bound.
+      + by apply gen_ns_sub_upto.
+      + cbn. set_solver. }
+    wp_apply (Thunks.force_spec _ p (gen_ns id) with "HtickInv [$TC $H $Hthunk $Hgens]").
+      by auto.
+    iIntros (?) "(? & ? & Hthunk & Hgens)". iApply "HΦ". iFrame.
+    iDestruct (na_own_union with "[$Hgens $Hthunk]") as "?". set_solver. done.
+  Qed.
+
+End Gthunks.
